Primitive_Matchers/IPPortIfaceSpace_Syntax.thy
@@ -15,14 +15,14 @@ text{*Primitive Match Conditions which only support interfaces, IPv4 addresses, 
 type_synonym ipt_ports = "(16 word \<times> 16 word) list"
 
 
-datatype_new ipportiface_rule_match = Src ipt_ipv4range | Dst ipt_ipv4range | IIface iface | OIface iface | Prot protocol | 
+datatype_new common_primitive = Src ipt_ipv4range | Dst ipt_ipv4range | IIface iface | OIface iface | Prot protocol | 
   is_Src_Ports: Src_Ports (src_ports_sel: ipt_ports) | 
   is_Dst_Ports: Dst_Ports (dst_ports_sel: ipt_ports) | 
   Extra string
 
 
 
-lemma wf_disc_sel_ipportiface_rule_match[simp]: 
+lemma wf_disc_sel_common_primitive[simp]: 
       "wf_disc_sel (is_Src_Ports, src_ports_sel) Src_Ports"
       "wf_disc_sel (is_Dst_Ports, dst_ports_sel) Dst_Ports"
   by(simp_all add: wf_disc_sel.simps)
